\subsection{Proof of Theorem 2.1: Consistency of Pooled OLS}

Under assumption $\mathcal{P}$, $\hat\theta_{pool}$ is identified as:
\begin{align*}
    \hat\theta_{pool} = (\sumt \sumi  x_{it}x_{it}')^{-1}\sumi\sumt x_{it}y_{it}
\end{align*}
When we plug in the model $y_{it} =  x_{it}'\theta + e_{it}$:

\begin{align*}
    \hat\theta_{pool} = (\sumt \sumi x_{it}x_{it}')^{-1}\sumt\sumi x_{it}x_{it}'\theta + (\sumt \sumi x_{it}x_{it}')^{-1} \sumt \sumi  x_{it}e_{it} \\
    = \theta + (\sumt \sumi x_{it}x_{it}')^{-1} \sumt \sumi x_{it}e_{it}\\
    = \theta + (\sumt \dfrac{1}{N} \sumi  x_{it}x_{it}')^{-1} \sumt \dfrac{1}{N} \sumi x_{it}e_{it}
\end{align*}
By assumption $\mathcal{P}$-1 and WLLN for i.i.d. random variables as N $\rightarrow \infty$:
\begin{align*}
\sumt \dfrac{1}{N} \sumi x_{it}x_{it}'  \overset{p}{\to} \EX(x_{it}x_{it}') \\
\sumt \dfrac{1}{N} \sumi x_{it}e_{it}  \overset{p}{\to} \EX(x_{it}e_{it}) 
\end{align*}

By assumption $\mathcal{P}$-2 $\EX(x_{it}e_{it}) = 0$.
Thus:
\begin{align*}
 \hat\theta_{pool} \overset{p}{\to} \theta + \EX(x_{it}x_{it}')^{-1}  \EX(x_{it}e_{it})\\
 \overset{p}{\to} \theta + \EX(x_{it}x_{it}')^{-1}0\\
 \overset{p}{\to} \theta 
\end{align*}
This shows that $\hat\theta_{pool}$ is a consistent estimator of $\theta$ when assumption $\mathcal{P}$ holds. 